new/golang/defn/pkg.v
@@ -4,8 +4,8 @@ From Perennial Require Import base.
 (** [PkgInfo] associates a pkg_name to its static information. *)
 Class PkgInfo (pkg_name: go_string) `{ffi_syntax} := {
     pkg_vars : list (go_string * go_type);
-    pkg_functions : list (go_string * val);
-    pkg_msets : list (go_string * (list (go_string * val)));
+    pkg_functions : go_string → val → bool;
+    pkg_msets : go_string → list (go_string * val) → bool;
     pkg_imported_pkgs : list go_string;
   }.
 
@@ -33,7 +33,6 @@ Module globals.
 Section defns.
 Context `{ffi_syntax}.
 
-Locate "#".
 Definition get_def : val :=
   λ: "var_name", (option.unwrap $ GlobalGet (#"V" + "var_name")).
 Program Definition get := sealed @get_def.
